examples/LinearSequence.s.dfy
@@ -1,11 +1,21 @@
-include "../lib/Base/sequences.i.dfy"
-
 include "LinearMaybe.s.dfy"
-
-import opened Sequences
 
 // module LinearSequence {
   // import opened LinearMaybe
+
+  function method seq_get<A>(shared s:seq<A>, i:nat):(a:A)
+      requires i < |s|
+      ensures a == s[i]
+  function method seq_set<A>(linear s1:seq<A>, i:nat, a:A):(linear s2:seq<A>) // can be implemented as in-place update
+      requires i < |s1|
+      ensures s2 == s1[i := a]
+  function method seq_length<A>(shared s:seq<A>):(n:nat)
+      ensures n == |s|
+
+  method seq_alloc<A>(length:nat) returns(linear s:seq<A>)
+      ensures |s| == length
+
+  method seq_free<A>(linear s:seq<A>)
 
   type lseq<A>
   function lseqs<A>(s:lseq<A>):seq<maybe<A>> // contents of an lseq, as ghost seq
@@ -28,49 +38,5 @@ import opened Sequences
   function method lseq_share<A>(shared s:lseq<A>, i:nat):(shared a:maybe<A>)
       requires i < |lseqs(s)|
       ensures a == lseqs(s)[i]
-
-  function method lseq_peek<A>(shared s:lseq<A>, i:nat):(shared a:A)
-      requires i < |lseqs(s)|
-      requires has(lseqs(s)[i])
-      ensures a == peek(lseqs(s)[i])
-  {
-      peek(lseq_share(s, i))
-  }
-
-  method lseq_get<A>(linear s1:lseq<A>, i:nat) returns(linear s2:lseq<A>, linear a:A)
-      requires i < |lseqs(s1)|
-      requires has(lseqs(s1)[i])
-      ensures a == read(lseqs(s1)[i])
-      ensures lseqs(s2) == lseqs(s1)[i := empty()]
-  {
-      linear var x1:maybe<A> := empty();
-      linear var x2:maybe<A>;
-      s2, x2 := lseq_swap(s1, i, x1);
-      a := unwrap(x2);
-  }
-
-  method lseq_set<A>(linear s1:lseq<A>, i:nat, linear a:A) returns(linear s2:lseq<A>)
-      requires i < |lseqs(s1)|
-      requires !has(lseqs(s1)[i])
-      ensures lseqs(s2) == lseqs(s1)[i := give(a)]
-  {
-      linear var x1:maybe<A> := give(a);
-      linear var x2:maybe<A>;
-      s2, x2 := lseq_swap(s1, i, x1);
-      var _ := discard(x2);
-  }
-
-  predicate lseq_full<A>(s: lseq<A>)
-  {
-      && (forall i | 0 <= i < lseq_length(s) :: has(lseqs(s)[i]))
-  }
-
-  function lseqs_full<A>(s: lseq<A>): (result: seq<A>)
-      requires lseq_full(s)
-      ensures |result| == lseq_length(s)
-      ensures forall i | 0 <= i < lseq_length(s) :: result[i] == peek(lseqs(s)[i])
-  {
-      Apply(x requires has(x) => peek(x), lseqs(s))
-  }
 
 // } // module
