examples/LinearSequence.i.dfy
@@ -1,0 +1,72 @@
+include "../lib/Base/sequences.i.dfy"
+
+include "LinearMaybe.s.dfy"
+include "LinearSequence.s.dfy"
+
+import opened Sequences
+
+// module LinearSequence_i {
+  // import opened LinearMaybe
+  // import opened LinearSequence
+
+  method seq_alloc_init<A>(length:nat, a:A) returns(linear s:seq<A>)
+      ensures |s| == length
+      ensures forall i:nat | i < |s| :: s[i] == a
+  {
+      s := seq_alloc(length);
+      var n := 0;
+      while (n < length)
+          invariant |s| == length;
+          invariant n <= length;
+          invariant forall i:nat | i < n :: s[i] == a
+      {
+          s := seq_set(s, n, a);
+          n := n + 1;
+      }
+  }
+
+  function method lseq_peek<A>(shared s:lseq<A>, i:nat):(shared a:A)
+      requires i < |lseqs(s)|
+      requires has(lseqs(s)[i])
+      ensures a == peek(lseqs(s)[i])
+  {
+      peek(lseq_share(s, i))
+  }
+
+  method lseq_take<A>(linear s1:lseq<A>, i:nat) returns(linear s2:lseq<A>, linear a:A)
+      requires i < |lseqs(s1)|
+      requires has(lseqs(s1)[i])
+      ensures a == read(lseqs(s1)[i])
+      ensures lseqs(s2) == lseqs(s1)[i := empty()]
+  {
+      linear var x1:maybe<A> := empty();
+      linear var x2:maybe<A>;
+      s2, x2 := lseq_swap(s1, i, x1);
+      a := unwrap(x2);
+  }
+
+  method lseq_give<A>(linear s1:lseq<A>, i:nat, linear a:A) returns(linear s2:lseq<A>)
+      requires i < |lseqs(s1)|
+      requires !has(lseqs(s1)[i])
+      ensures lseqs(s2) == lseqs(s1)[i := give(a)]
+  {
+      linear var x1:maybe<A> := give(a);
+      linear var x2:maybe<A>;
+      s2, x2 := lseq_swap(s1, i, x1);
+      var _ := discard(x2);
+  }
+
+  predicate lseq_full<A>(s: lseq<A>)
+  {
+      && (forall i | 0 <= i < lseq_length(s) :: has(lseqs(s)[i]))
+  }
+
+  function{:opaque} lseqs_full<A>(s: lseq<A>): (result: seq<A>)
+      requires lseq_full(s)
+      ensures |result| == lseq_length(s)
+      ensures forall i | 0 <= i < lseq_length(s) :: result[i] == peek(lseqs(s)[i])
+  {
+      Apply(x requires has(x) => peek(x), lseqs(s))
+  }
+
+// } // module
